fiat2/src/fiat2/IndexTransf2.v
@@ -1,0 +1,187 @@
+Require Import fiat2.Language fiat2.Interpret fiat2.Value fiat2.TypeSystem fiat2.TypeSound fiat2.IndexInterface2
+  fiat2.Utils fiat2.TransfSound fiat2.Substitute.
+Require Import coqutil.Map.Interface coqutil.Word.Interface coqutil.Datatypes.Result.
+Require Import List String ZArith Sorted Permutation.
+Import ListNotations.
+
+Fixpoint mk_compo_idx' (e : expr) (free_vars : list string) (idxs : list (string * IndexInterface2.index)) :=
+  match idxs with
+  | nil => nil
+  | (tag, idx) :: idxs => (tag, substitute [(@hole idx, e)] free_vars (@to_idx idx)) :: mk_compo_idx' e free_vars idxs
+  end.
+
+Definition mk_compo_idx (e : expr) (free_vars : list string) (idxs : list (string * IndexInterface2.index)) :=
+  ERecord (mk_compo_idx' e free_vars idxs).
+
+Lemma map_fst_map_triple : forall A B C D (l : list (A * B * C)) (f : B -> D),
+    List.map fst (List.map (fun '(a, b, _) => (a, f b)) l) = List.map fst (List.map fst l).
+Proof.
+  intros; induction l; cbn; auto.
+  repeat case_match; cbn; congruence.
+Qed.
+
+Section compo_idx.
+  Section WithMap.
+    Context {tenv : map.map string type} {tenv_ok : map.ok tenv}.
+    Context {width: Z} {word: word.word width} {word_ok: word.ok word}.
+    Notation value := (value (width:=width)).
+    Context {locals : map.map string value} {locals_ok : map.ok locals}.
+
+    Context (idxs : list (string * IndexInterface2.index * (value -> value -> Prop))).
+    Context (idxs_ok : Forall (fun '(_, idx, idx_wf) => ok idx idx_wf) idxs).
+    Context (H_tag_NoDup : NoDup (List.map fst (List.map fst idxs))).
+    Context (hole0 : string).
+    Context (H_holes_eq : Forall (fun '(_, idx, _) => @hole idx = hole0) idxs).
+
+    Definition compo_idx_ty (t : type) : type :=
+      TRecord (record_sort (List.map (fun '(tag, idx, _) => (tag, @idx_ty idx t)) idxs)).
+
+    Definition to_compo_idx : expr :=
+      ERecord (List.map (fun '(tag, idx, _) => (tag, @to_idx idx)) idxs).
+
+    Definition compo_idx_wf (v v' : value) : Prop :=
+      match v' with
+      | VRecord v' =>
+          Forall (fun '(tag, _, idx_wf) => idx_wf v (record_proj tag v')) idxs
+      | _ => False
+      end.
+
+    Definition compo_is_tbl_ty (t : type) : bool :=
+      forallb (fun '(tag, idx, _) => @is_tbl_ty idx t) idxs.
+
+    Lemma to_compo_idx_ty : forall (t : type),
+        type_wf t -> compo_is_tbl_ty t = true ->
+        type_of map.empty (map.put map.empty hole0 t) to_compo_idx (compo_idx_ty t).
+    Proof.
+      unfold compo_is_tbl_ty, to_compo_idx, compo_idx_ty.
+      intros. econstructor; eauto using Permuted_record_sort, StronglySorted_record_sort.
+      1:{ clear. induction idxs; cbn; auto.
+          do 2 case_match; cbn; congruence. }
+      1:{ induction idxs; auto. cbn in *.
+          repeat invert_Forall; invert_NoDup; rewrite Bool.andb_true_iff in *; intuition idtac.
+          constructor; auto.
+          do 2 case_match; cbn; subst. eapply (to_idx_ty (idx:=i)); eauto. }
+      1:{ revert H_tag_NoDup; clear; intros.
+          induction idxs; intros; cbn; auto using NoDup_nil.
+          cbn in *; invert_NoDup.
+          constructor; auto. do 2 case_match; cbn in *.
+          rewrite map_fst_map_triple; auto. }
+    Qed.
+
+    Lemma compo_idx_ty_wf : forall t : type,
+        type_wf t -> compo_is_tbl_ty t = true ->
+        type_wf (compo_idx_ty t).
+    Proof.
+      unfold compo_is_tbl_ty, compo_idx_ty; intros ? ? H.
+      eapply List.forallb_to_Forall with (P:=fun '(_, idx, _) => @is_tbl_ty idx t = true) in H.
+      2: intros; repeat case_match; auto.
+      constructor; auto using StronglySorted_record_sort.
+      1:{ eapply Permutation_NoDup.
+          1: apply Permutation_map, Permuted_record_sort.
+          induction idxs; cbn in *; auto.
+          repeat invert_Forall; invert_NoDup.
+          constructor; auto.
+          repeat case_match; cbn in *.
+          rewrite map_fst_map_triple; auto. }
+      1:{ rewrite Forall_map.
+          eapply Permutation_Forall.
+          1: apply Permuted_record_sort.
+          induction H; cbn in *; auto.
+          repeat invert_Forall; invert_NoDup.
+          constructor; repeat case_match; auto.
+          cbn; auto using idx_ty_wf. }
+    Qed.
+
+    Lemma NoDup_In_access_record : forall A (l : list (string * A)),
+        NoDup (List.map fst l) ->
+        forall s v, In (s, v) l ->
+        access_record l s = Success v.
+    Proof.
+      intros * ? ? ? H_in; induction l; cbn in *.
+      1: intuition fail.
+      do 2 case_match; rewrite ?eqb_eq, ?eqb_neq in *; invert_NoDup.
+      1:{ subst. intuition idtac; try congruence.
+          apply in_map with (f:=fst) in H0;
+            cbn in *; intuition idtac. }
+      1:{ intuition idtac. congruence. }
+    Qed.
+
+    Lemma NoDup_Permutation_access_record : forall s A (l l' : list (string * A)),
+        NoDup (List.map fst l) ->
+        In s (List.map fst l) ->
+        Permutation l l' ->
+        access_record l s = access_record l' s.
+    Proof.
+      intros * H_NoDup H_in H_permu.
+      apply In_access_record in H_in. destruct_exists.
+      rewrite_l_to_r.
+      apply access_record_sound in H.
+      symmetry. apply NoDup_In_access_record.
+      1:{ eapply Permutation_NoDup.
+          1: apply Permutation_map; eauto.
+          assumption. }
+      1:{ eapply Permutation_in; eauto. }
+    Qed.
+
+    Lemma to_compo_idx_wf : forall (v : value) (t : type),
+      type_wf t -> compo_is_tbl_ty t = true ->
+      type_of_value v t ->
+      compo_idx_wf v (interp_expr map.empty (map.put map.empty hole0 v) to_compo_idx).
+    Proof.
+      intros.
+      unfold compo_idx_wf, compo_idx_ty, to_compo_idx, compo_is_tbl_ty, record_proj in *.
+      cbn [interp_expr].
+      rewrite Forall_forall; intros. do 2 case_match.
+      erewrite NoDup_Permutation_access_record.
+      4: apply Permutation_sym, Permuted_record_sort.
+      2:{ eapply Permutation_NoDup.
+          1: eapply Permutation_map, Permuted_record_sort.
+          rewrite fst_map_fst, map_fst_map_triple; auto. }
+      2:{ rewrite in_map_iff. eexists; intuition idtac.
+          2:{ eapply Permutation_in.
+              1: apply Permuted_record_sort.
+              rewrite in_map_iff. exists (s, to_idx).
+              intuition idtac.
+              rewrite in_map_iff; exists x.
+              subst; auto. }
+          reflexivity. }
+      eapply List.forallb_to_Forall with (P:=fun '(_, idx, _) => @is_tbl_ty idx t = true) in H0.
+      2: intros; repeat case_match; auto.
+      repeat apply_Forall_In. cbn in *.
+      apply to_idx_wf in H1; auto.
+      erewrite NoDup_In_access_record; eauto.
+      2:{ erewrite in_map_iff. exists (s, to_idx).
+          subst; intuition auto.
+          erewrite in_map_iff. exists (s, i, P); auto. }
+      rewrite fst_map_fst, map_fst_map_triple; auto.
+    Qed.
+
+    Instance compo_idx : IndexInterface2.index := IndexInterface2.mk hole0 to_compo_idx compo_idx_ty compo_is_tbl_ty.
+
+    Instance compo_idx_ok : IndexInterface2.ok compo_idx compo_idx_wf :=
+      IndexInterface2.Build_ok compo_idx compo_idx_wf compo_idx_ty_wf to_compo_idx_ty to_compo_idx_wf.
+  End WithMap.
+End compo_idx.
+
+Section WithTags.
+  Context (id_tag aux_tag: string).
+  Context (tbl : string).
+  Context (idx : IndexInterface2.index).
+
+  Definition create_aux_write_head (free_vars : list string) (c : command) :=
+    match c with
+    | CAssign tbl' e =>
+        if String.eqb tbl tbl'
+        then CAssign tbl (ERecord [(id_tag, e); (aux_tag, substitute ((@hole idx, e) :: nil) free_vars (@to_idx idx))])
+        else c
+    | _ => c
+    end.
+
+  Definition create_aux_read_head (e : expr) :=
+    match e with
+    | ELoc x => if String.eqb tbl x
+                then (EAccess (ELoc tbl) id_tag)
+                else e
+    | _ => e
+    end.
+End WithTags.
